deduction system 2

Logic/Modal/Standard/Deduction.lean
@@ -7,26 +7,56 @@ namespace LO.Modal.Standard
 
 variable {α : Type*} [DecidableEq α]
 
-inductive Deduction (Λ : AxiomSet α) : (Formula α) → Type _
-  | maxm {p}     : p ∈ Λ → Deduction Λ p
-  | mdp {p q}    : Deduction Λ (p ⟶ q) → Deduction Λ p → Deduction Λ q
-  | nec {p}      : Deduction Λ p → Deduction Λ (□p)
-  | verum        : Deduction Λ ⊤
-  | imply₁ p q   : Deduction Λ (p ⟶ q ⟶ p)
-  | imply₂ p q r : Deduction Λ ((p ⟶ q ⟶ r) ⟶ (p ⟶ q) ⟶ p ⟶ r)
-  | conj₁ p q    : Deduction Λ (p ⋏ q ⟶ p)
-  | conj₂ p q    : Deduction Λ (p ⋏ q ⟶ q)
-  | conj₃ p q    : Deduction Λ (p ⟶ q ⟶ p ⋏ q)
-  | disj₁ p q    : Deduction Λ (p ⟶ p ⋎ q)
-  | disj₂ p q    : Deduction Λ (q ⟶ p ⋎ q)
-  | disj₃ p q r  : Deduction Λ ((p ⟶ r) ⟶ (q ⟶ r) ⟶ (p ⋎ q ⟶ r))
-  | dne p        : Deduction Λ (~~p ⟶ p)
+/--
+  Parameter for deduction system.
+-/
+structure DeductionParameter (α) where
+  axiomSet : AxiomSet α
+  nec : Bool
+notation:max "Ax(" L ")" => DeductionParameter.axiomSet L
 
-instance : System (Formula α) (AxiomSet α) := ⟨Deduction⟩
+namespace DeductionParameter
 
-open Deduction
+variable (L L₁ L₂ : DeductionParameter α)
 
-instance : System.Classical (Λ : AxiomSet α) where
+class HasNec where
+  has_nec : L.nec = true := by rfl
+
+class IncludeK where
+  include_K : 𝗞 ⊆ Ax(L) := by intro; aesop;
+
+/--
+  Deduction system of `L` is normal modal Logic.
+-/
+class Normal extends HasNec L, IncludeK L
+
+end DeductionParameter
+
+
+inductive Deduction (L : DeductionParameter α) : (Formula α) → Type _
+  | maxm {p}     : p ∈ Ax(L) → Deduction L p
+  | mdp {p q}    : Deduction L (p ⟶ q) → Deduction L p → Deduction L q
+  | nec {p}      : (L.nec = true) → Deduction L p → Deduction L (□p)
+  | verum        : Deduction L ⊤
+  | imply₁ p q   : Deduction L (p ⟶ q ⟶ p)
+  | imply₂ p q r : Deduction L ((p ⟶ q ⟶ r) ⟶ (p ⟶ q) ⟶ p ⟶ r)
+  | conj₁ p q    : Deduction L (p ⋏ q ⟶ p)
+  | conj₂ p q    : Deduction L (p ⋏ q ⟶ q)
+  | conj₃ p q    : Deduction L (p ⟶ q ⟶ p ⋏ q)
+  | disj₁ p q    : Deduction L (p ⟶ p ⋎ q)
+  | disj₂ p q    : Deduction L (q ⟶ p ⋎ q)
+  | disj₃ p q r  : Deduction L ((p ⟶ r) ⟶ (q ⟶ r) ⟶ (p ⋎ q ⟶ r))
+  | dne p        : Deduction L (~~p ⟶ p)
+
+namespace Deduction
+
+open DeductionParameter
+
+instance : System (Formula α) (DeductionParameter α) := ⟨Deduction⟩
+
+variable {L L₁ L₂ : DeductionParameter α}
+
+instance : System.Classical L where
   mdp := mdp
   verum := verum
   imply₁ := imply₁
@@ -39,15 +69,10 @@ instance : System.Classical (Λ : AxiomSet α) where
   disj₃ := disj₃
   dne := dne
 
-instance : System.Necessitation (Λ : AxiomSet α) where
-  nec := nec
-
-variable {Λ₁ Λ₂ : AxiomSet α}
-
-def maxm_subset (hs : Λ₁ ⊆ Λ₂) : (Λ₁ ⊢ p) → (Λ₂ ⊢ p)
-  | maxm h => maxm (hs h)
-  | mdp h₁ h₂    => mdp (maxm_subset hs h₁) (maxm_subset hs h₂)
-  | nec h        => nec $ maxm_subset hs h
+def maxm_subset (hNec : L₁.nec ≤ L₂.nec) (hAx : Ax(L₁) ⊆ Ax(L₂)) : (L₁ ⊢ p) → (L₂ ⊢ p)
+  | maxm h => maxm (hAx h)
+  | mdp ih₁ ih₂  => mdp (maxm_subset hNec hAx ih₁) (maxm_subset hNec hAx ih₂)
+  | nec p h      => nec (by aesop) $ maxm_subset hNec hAx h
   | verum        => verum
   | imply₁ _ _   => imply₁ _ _
   | imply₂ _ _ _ => imply₂ _ _ _
@@ -59,11 +84,45 @@ def maxm_subset (hs : Λ₁ ⊆ Λ₂) : (Λ₁ ⊢ p) → (Λ₂ ⊢ p)
   | disj₃ _ _ _  => disj₃ _ _ _
   | dne _        => dne _
 
-lemma maxm_subset! (hs : Λ₁ ⊆ Λ₂) (h : Λ₁ ⊢! p) : Λ₂ ⊢! p := ⟨maxm_subset hs h.some⟩
+lemma maxm_subset! (hNec : L₁.nec ≤ L₂.nec) (hAx : Ax(L₁) ⊆ Ax(L₂)) (h : L₁ ⊢! p) : L₂ ⊢! p := ⟨maxm_subset hNec hAx h.some⟩
 
-instance K_of_subset_K (hK : 𝐊 ⊆ Λ := by simp) : System.K (Λ : AxiomSet α) where
-  K _ _ := maxm $ Set.mem_of_subset_of_mem hK (by simp);
+@[simp]
+lemma reducible_of_subset (hNec : L₁.nec ≤ L₂.nec) (hAx : Ax(L₁) ⊆ Ax(L₂) := by intro; aesop) : L₁ ≤ₛ L₂ := by
+  intro p hp;
+  apply maxm_subset! hNec hAx hp;
 
+instance [HasNec L] : System.Necessitation L where
+  nec := nec HasNec.has_nec
+
+instance [IncludeK L] : System.HasAxiomK L where
+  K _ _ := maxm $ Set.mem_of_subset_of_mem (IncludeK.include_K) (by simp);
+
+instance [Normal L] : System.K L where
+
+lemma inducition_with_nec [HasNec L]
+  {motive  : (p : Formula α) → Deduction L p → Sort*}
+  (hMaxm   : ∀ {p}, (h : p ∈ Ax(L)) → motive p (maxm h))
+  (hMdp    : ∀ {p q}, (hpq : L ⊢ p ⟶ q) → (hp : L ⊢ p) → motive (p ⟶ q) hpq → motive p hp → motive q (hpq ⨀ hp))
+  (hNec    : ∀ {p}, (hp : L ⊢ p) → motive p hp → motive (□p) (nec HasNec.has_nec hp))
+  (hVerum  : motive ⊤ verum)
+  (hImply₁ : ∀ {p q}, motive (p ⟶ q ⟶ p) $ imply₁ p q)
+  (hImply₂ : ∀ {p q r}, motive ((p ⟶ q ⟶ r) ⟶ (p ⟶ q) ⟶ p ⟶ r) $ imply₂ p q r)
+  (hConj₁  : ∀ {p q}, motive (p ⋏ q ⟶ p) $ conj₁ p q)
+  (hConj₂  : ∀ {p q}, motive (p ⋏ q ⟶ q) $ conj₂ p q)
+  (hConj₃  : ∀ {p q}, motive (p ⟶ q ⟶ p ⋏ q) $ conj₃ p q)
+  (hDisj₁  : ∀ {p q}, motive (p ⟶ p ⋎ q) $ disj₁ p q)
+  (hDisj₂  : ∀ {p q}, motive (q ⟶ p ⋎ q) $ disj₂ p q)
+  (hDisj₃  : ∀ {p q r}, motive ((p ⟶ r) ⟶ (q ⟶ r) ⟶ (p ⋎ q ⟶ r)) $ disj₃ p q r)
+  (hDne    : ∀ {p}, motive (~~p ⟶ p) $ dne p)
+  : ∀ {p}, (d : L ⊢ p) → motive p d := by
+  intro p d;
+  induction d with
+  | maxm h => exact hMaxm h
+  | mdp hpq hp ihpq ihp => exact hMdp hpq hp ihpq ihp
+  | nec _ hp ihp => exact hNec hp ihp
+  | _ => aesop
+
+/-
 instance : System.K (𝐊 : AxiomSet α) := K_of_subset_K (by rfl)
 
 instance : System.K (𝐊 ∪ Λ : AxiomSet α) := K_of_subset_K
@@ -74,5 +133,101 @@ instance S4_of_subset_S4 (hS4 : 𝐒𝟒 ⊆ Λ := by simp) : System.S4 (Λ : Ax
   Four _  := Deduction.maxm $ Set.mem_of_subset_of_mem hS4 (by simp);
 
 instance : System.S4 (𝐒𝟒 : AxiomSet α) := S4_of_subset_S4 (by rfl)
+-/
+
+end Deduction
+
+
+namespace DeductionParameter
+
+open DeductionParameter
+
+private abbrev NecOnly (Ax : AxiomSet α) : DeductionParameter α where
+  axiomSet := Ax
+  nec := true
+
+protected abbrev K : DeductionParameter α := NecOnly 𝗞
+notation "𝐊" => DeductionParameter.K
+instance : Normal (α := α) 𝐊 where
+
+
+protected abbrev KT : DeductionParameter α := NecOnly (𝗞 ∪ 𝗧)
+notation "𝐊𝐓" => DeductionParameter.KT
+instance : Normal (α := α) 𝐊𝐓 where
+
+
+protected abbrev KD : DeductionParameter α := NecOnly (𝗞 ∪ 𝗗)
+notation "𝐊𝐃" => DeductionParameter.KD
+instance : Normal (α := α) 𝐊𝐃 where
+
+
+protected abbrev K4 : DeductionParameter α := NecOnly (𝗞 ∪ 𝟰)
+notation "𝐊𝟒" => DeductionParameter.K4
+instance : Normal (α := α) 𝐊𝟒 where
+
+
+protected abbrev K5 : DeductionParameter α := NecOnly (𝗞 ∪ 𝟱)
+notation "𝐊𝟓" => DeductionParameter.K5
+instance : Normal (α := α) 𝐊𝟓 where
+
+
+protected abbrev S4 : DeductionParameter α := NecOnly (𝗞 ∪ 𝗧 ∪ 𝟰)
+notation "𝐒𝟒" => DeductionParameter.S4
+instance : Normal (α := α) 𝐒𝟒 where
+
+instance : System.S4 (𝐒𝟒 : DeductionParameter α) where
+  T _ := Deduction.maxm $ Set.mem_of_subset_of_mem (by rfl) (by simp)
+  Four _ := Deduction.maxm $ Set.mem_of_subset_of_mem (by rfl) (by simp)
+
+
+protected abbrev S5 : DeductionParameter α := NecOnly (𝗞 ∪ 𝗧 ∪ 𝟱)
+notation "𝐒𝟓" => DeductionParameter.S5
+instance : Normal (α := α) 𝐒𝟓 where
+
+
+protected abbrev KT4B : DeductionParameter α := NecOnly (𝗞 ∪ 𝗧 ∪ 𝟰 ∪ 𝗕)
+notation "𝐊𝐓𝟒𝐁" => DeductionParameter.KT4B
+instance : Normal (α := α) 𝐊𝐓𝟒𝐁 where
+
+
+protected abbrev GL : DeductionParameter α := NecOnly (𝗞 ∪ 𝗟)
+notation "𝐆𝐋" => DeductionParameter.GL
+instance : Normal (α := α) 𝐆𝐋 where
+
+
+protected abbrev S4Dot2 : DeductionParameter α := NecOnly (𝗞 ∪ 𝗧 ∪ 𝟰 ∪ .𝟮)
+notation "𝐒𝟒.𝟐" => DeductionParameter.S4Dot2
+instance : Normal (α := α) 𝐒𝟒.𝟐 where
+
+
+protected abbrev S4Dot3 : DeductionParameter α := NecOnly (𝗞 ∪ 𝗧 ∪ 𝟰 ∪ .𝟯)
+notation "𝐒𝟒.𝟑" => DeductionParameter.S4Dot3
+instance : Normal (α := α) 𝐒𝟒.𝟑 where
+
+
+protected abbrev S4Grz : DeductionParameter α := NecOnly (𝗞 ∪ 𝗧 ∪ 𝟰 ∪ 𝗚𝗿𝘇)
+notation "𝐒𝟒𝐆𝐫𝐳" => DeductionParameter.S4Grz
+instance : Normal (α := α) 𝐒𝟒𝐆𝐫𝐳 where
+
+
+/-- Logic of Pure Necessitation -/
+protected abbrev N : DeductionParameter α := NecOnly ∅
+notation "𝐍" => DeductionParameter.N
+
+end DeductionParameter
+
+@[simp] lemma reducible_K_KT : (𝐊 : DeductionParameter α) ≤ₛ 𝐊𝐓 := by simp
+
+@[simp] lemma reducible_K_KD : (𝐊 : DeductionParameter α) ≤ₛ 𝐊𝐃 := by simp
+
+@[simp] lemma reducible_KT_S4 : (𝐊𝐓 : DeductionParameter α) ≤ₛ 𝐒𝟒 := by simp
+
+@[simp] lemma reducible_S4_S4Dot2 : (𝐒𝟒 : DeductionParameter α) ≤ₛ 𝐒𝟒.𝟐 := by simp
+
+@[simp] lemma reducible_S4_S4Dot3 : (𝐒𝟒 : DeductionParameter α) ≤ₛ 𝐒𝟒.𝟑 := by simp
+
+@[simp] lemma reducible_S4_S4Grz : (𝐒𝟒 : DeductionParameter α) ≤ₛ 𝐒𝟒𝐆𝐫𝐳 := by simp
+
+@[simp] lemma reducible_K_GL : (𝐊 : DeductionParameter α) ≤ₛ 𝐆𝐋 := by simp
 
 end LO.Modal.Standard
