Logic/Modal/Standard/Geach.lean
@@ -18,84 +18,104 @@ end LO.System.Axioms
 
 namespace LO.Modal.Standard
 
-variable {Λ : AxiomSet α}
+variable {Ax : AxiomSet α}
 
 open System
 
 namespace AxiomSet
 
 abbrev Geach (l : Axioms.Geach.Taple) : AxiomSet α := { Axioms.Geach l p | (p) }
-notation:max "𝐠𝐞(" t ")" => AxiomSet.Geach t
+notation:max "𝗴𝗲(" t ")" => AxiomSet.Geach t
 
-class IsGeach (Λ : AxiomSet α) where
+class IsGeach (Ax : AxiomSet α) where
   taple : Axioms.Geach.Taple
-  char : Λ = AxiomSet.Geach taple := by rfl
+  char : Ax = AxiomSet.Geach taple := by rfl
 
-instance : IsGeach (α := α) 𝐓 where taple := ⟨0, 0, 1, 0⟩;
+instance : IsGeach (α := α) 𝗧 where taple := ⟨0, 0, 1, 0⟩;
 
-instance : IsGeach (α := α) 𝐁 where taple := ⟨0, 1, 0, 1⟩;
+instance : IsGeach (α := α) 𝗕 where taple := ⟨0, 1, 0, 1⟩;
 
-instance : IsGeach (α := α) 𝐃 where taple := ⟨0, 0, 1, 1⟩;
+instance : IsGeach (α := α) 𝗗 where taple := ⟨0, 0, 1, 1⟩;
 
-instance : IsGeach (α := α) 𝟒 where taple := ⟨0, 2, 1, 0⟩;
+instance : IsGeach (α := α) 𝟰 where taple := ⟨0, 2, 1, 0⟩;
 
-instance : IsGeach (α := α) 𝟓 where taple := ⟨1, 1, 0, 1⟩;
+instance : IsGeach (α := α) 𝟱 where taple := ⟨1, 1, 0, 1⟩;
 
-instance : IsGeach (α := α) .𝟐 where taple := ⟨1, 1, 1, 1⟩;
+instance : IsGeach (α := α) .𝟮 where taple := ⟨1, 1, 1, 1⟩;
 
-instance : IsGeach (α := α) 𝐂𝟒 where taple := ⟨0, 1, 2, 0⟩;
+instance : IsGeach (α := α) 𝗖𝟰 where taple := ⟨0, 1, 2, 0⟩;
 
-instance : IsGeach (α := α) 𝐂𝐃 where taple := ⟨1, 1, 0, 0⟩;
+instance : IsGeach (α := α) 𝗖𝗗 where taple := ⟨1, 1, 0, 0⟩;
 
 
-def GeachLogic : List Axioms.Geach.Taple → AxiomSet α
-  | [] => 𝐊
-  | x :: xs => (AxiomSet.Geach x) ∪ (AxiomSet.GeachLogic xs)
-notation:max "𝐆𝐞(" l ")" => AxiomSet.GeachLogic l
+def MultiGeach : List Axioms.Geach.Taple → AxiomSet α
+  | [] => 𝗞
+  | x :: xs => (AxiomSet.Geach x) ∪ (AxiomSet.MultiGeach xs)
+notation:max "𝗚𝗲(" l ")" => AxiomSet.MultiGeach l
 
-namespace GeachLogic
-
-@[simp]
-lemma def_nil : 𝐆𝐞([]) = (𝐊 : AxiomSet α) := by simp [GeachLogic]
+namespace MultiGeach
 
 @[simp]
-lemma iff_cons : 𝐆𝐞(x :: l) = (𝐠𝐞(x) : AxiomSet α) ∪ 𝐆𝐞(l) := by simp only [GeachLogic];
+lemma def_nil : 𝗚𝗲([]) = (𝗞 : AxiomSet α) := by simp [MultiGeach]
 
 @[simp]
-lemma subsetK : (𝐊 : AxiomSet α) ⊆ 𝐆𝐞(l) := by
+lemma iff_cons : 𝗚𝗲(x :: l) = (𝗴𝗲(x) : AxiomSet α) ∪ 𝗚𝗲(l) := by simp only [MultiGeach];
+
+@[simp]
+lemma subsetK : (𝗞 : AxiomSet α) ⊆ 𝗚𝗲(l) := by
   induction l with
   | nil => simp;
   | cons => simp; apply Set.subset_union_of_subset_right (by assumption);
 
-lemma subsetK' (h : 𝐆𝐞(l) ⊆ Λ): 𝐊 ⊆ Λ := Set.Subset.trans GeachLogic.subsetK h
+lemma subsetK' (h : 𝗚𝗲(l) ⊆ Ax): 𝗞 ⊆ Ax := Set.Subset.trans subsetK h
 
-instance instK : System.K (𝐆𝐞(l) : AxiomSet α) := K_of_subset_K (by simp)
+-- instance instK : System.K (𝐆𝐞(l) : AxiomSet α) := K_of_subset_K (by simp)
 
-end GeachLogic
-
-class IsGeachLogic (Λ : AxiomSet α) where
-  taples : List Axioms.Geach.Taple
-  char : Λ = 𝐆𝐞(taples) := by aesop;
-
-instance [Λ.IsGeachLogic] : System.K Λ := by rw [IsGeachLogic.char (Λ := Λ)]; exact GeachLogic.instK;
-
-instance : IsGeachLogic (α := α) 𝐊 where taples := [];
-
-instance : IsGeachLogic (α := α) 𝐊𝐃 where taples := [⟨0, 0, 1, 1⟩]
-
-instance : IsGeachLogic (α := α) 𝐊𝐓 where taples := [⟨0, 0, 1, 0⟩]
-
-instance : IsGeachLogic (α := α) 𝐊𝟒 where taples := [⟨0, 2, 1, 0⟩]
-
-instance : IsGeachLogic (α := α) 𝐒𝟒 where taples := [⟨0, 0, 1, 0⟩, ⟨0, 2, 1, 0⟩]
-
-instance : IsGeachLogic (α := α) 𝐒𝟒.𝟐 where taples := [⟨0, 0, 1, 0⟩, ⟨0, 2, 1, 0⟩, ⟨1, 1, 1, 1⟩]
-
-instance : IsGeachLogic (α := α) 𝐒𝟓 where taples := [⟨0, 0, 1, 0⟩, ⟨1, 1, 0, 1⟩]
-
-instance : IsGeachLogic (α := α) 𝐊𝐓𝟒𝐁 where taples := [⟨0, 0, 1, 0⟩, ⟨0, 2, 1, 0⟩, ⟨0, 1, 0, 1⟩]
+end MultiGeach
 
 end AxiomSet
 
+
+namespace DeductionParameter
+
+protected abbrev Geach (l : List Axioms.Geach.Taple) : DeductionParameter α where
+  axiomSet := 𝗚𝗲(l)
+  nec := true
+notation "𝐆𝐞(" l ")" => DeductionParameter.Geach l
+instance instNormal : Normal (α := α) 𝐆𝐞(l) where
+  include_K := by simp [AxiomSet.MultiGeach.subsetK]
+
+protected class IsGeach (L : DeductionParameter α) where
+  taples : List Axioms.Geach.Taple
+  char : L = 𝐆𝐞(taples) := by aesop;
+
+namespace IsGeach
+
+variable {L : DeductionParameter α} [geach : L.IsGeach]
+
+instance : L.Normal := by
+  rw [geach.char];
+  infer_instance
+
+@[simp]
+lemma eq_axiomset : Ax(L) = 𝗚𝗲(IsGeach.taples L) := by have := geach.char; simp_all;
+
+instance : DeductionParameter.IsGeach (α := α) 𝐊 where taples := [];
+
+instance : DeductionParameter.IsGeach (α := α) 𝐊𝐃 where taples := [⟨0, 0, 1, 1⟩]
+
+instance : DeductionParameter.IsGeach (α := α) 𝐊𝐓 where taples := [⟨0, 0, 1, 0⟩]
+
+instance : DeductionParameter.IsGeach (α := α) 𝐒𝟒 where taples := [⟨0, 0, 1, 0⟩, ⟨0, 2, 1, 0⟩]
+
+instance : DeductionParameter.IsGeach (α := α) 𝐒𝟒.𝟐 where taples := [⟨0, 0, 1, 0⟩, ⟨0, 2, 1, 0⟩, ⟨1, 1, 1, 1⟩]
+
+instance : DeductionParameter.IsGeach (α := α) 𝐒𝟓 where taples := [⟨0, 0, 1, 0⟩, ⟨1, 1, 0, 1⟩]
+
+instance : DeductionParameter.IsGeach (α := α) 𝐊𝐓𝟒𝐁 where taples := [⟨0, 0, 1, 0⟩, ⟨0, 2, 1, 0⟩, ⟨0, 1, 0, 1⟩]
+
+end IsGeach
+
+end DeductionParameter
 
 end LO.Modal.Standard
