Logic/Modal/Standard/Kripke/Semantics.lean
@@ -10,7 +10,7 @@ namespace Kripke
 -- variable (W α : Type*) [Inhabited W]
 
 set_option linter.unusedVariables false in
-abbrev Frame (W : Sort*) (α : Type*) [Inhabited W] := W → W → Prop
+abbrev Frame (W) (α : Type*) [Inhabited W] := W → W → Prop
 
 @[simp]
 def Multiframe {W α} [Inhabited W] (F : Frame W α) : ℕ → W → W → Prop
@@ -165,8 +165,8 @@ namespace Formula.Kripke.ValidOnFrameClass
 
 end Formula.Kripke.ValidOnFrameClass
 
-def Kripke.AxiomSetFrameClass (Λ : AxiomSet α) : FrameClass α := λ _ _ F => F ⊧* Λ
-notation "𝔽(" Λ ")" => Kripke.AxiomSetFrameClass Λ
+def Kripke.AxiomSetFrameClass (Ax : AxiomSet α) : FrameClass α := λ _ _ F => F ⊧* Ax
+notation "𝔽(" Ax ")" => Kripke.AxiomSetFrameClass Ax
 
 
 @[simp] def Formula.Kripke.ValidOnFiniteFrameClass (𝔽 : FiniteFrameClass α) (f : Formula α) := ∀ W, [Inhabited W] → [Finite W] → ∀ F, 𝔽 W F → F ⊧ f
@@ -179,24 +179,23 @@ namespace Formula.Kripke.ValidOnFiniteFrameClass
 
 end Formula.Kripke.ValidOnFiniteFrameClass
 
-def Kripke.AxiomSetFiniteFrameClass (Λ : AxiomSet α) : FiniteFrameClass α := λ _ _ _ F => F ⊧* Λ
-notation "𝔽ꟳ(" Λ ")" => Kripke.AxiomSetFiniteFrameClass Λ
+def Kripke.AxiomSetFiniteFrameClass (Ax : AxiomSet α) : FiniteFrameClass α := λ _ _ _ F => F ⊧* Ax
+notation "𝔽ꟳ(" Ax ")" => Kripke.AxiomSetFiniteFrameClass Ax
 
+variable {Ax : AxiomSet α}
 
 namespace Kripke
 
-variable {Λ : AxiomSet α}
-
-lemma validOnAxiomSetFrameClass_axiom (h : p ∈ Λ) : 𝔽(Λ) ⊧ p := by
+lemma validOnAxiomSetFrameClass_axiom (h : p ∈ Ax) : 𝔽(Ax) ⊧ p := by
   intro _ _ _ hF;
   exact hF.realize h;
 
 
-/-- Every frame that valid all axioms in `Λ` satisfy frame property `P` -/
-class Definability (Λ : AxiomSet α) (P : FrameProperty α) where
-  defines : ∀ W, [Inhabited W] → ∀ F, F ⊧* Λ ↔ @P W _ F
+/-- Every frame that valid all axioms in `Ax` satisfy frame property `P` -/
+class Definability (Ax : AxiomSet α) (P : FrameProperty α) where
+  defines : ∀ W, [Inhabited W] → ∀ F, F ⊧* Ax ↔ @P W _ F
 
-instance Definability.union [definability₁ : Definability Λ₁ P₁] [definability₂ : Definability Λ₂ P₂] : Definability (Λ₁ ∪ Λ₂) (λ F => P₁ F ∧ P₂ F) where
+instance Definability.union [definability₁ : Definability Ax₁ P₁] [definability₂ : Definability Ax₂ P₂] : Definability (Ax₁ ∪ Ax₂) (λ F => P₁ F ∧ P₂ F) where
   defines W _ F := by
     constructor;
     . intro h;
@@ -210,15 +209,15 @@ instance Definability.union [definability₁ : Definability Λ₁ P₁] [definab
       . apply Definability.defines W F |>.mpr h.1;
       . apply Definability.defines W F |>.mpr h.2;
 
-lemma iff_definability_memAxiomSetFrameClass (definability : Definability Λ P) : ∀ {W}, [Inhabited W] → ∀ {F}, 𝔽(Λ) W F ↔ P F := by
+lemma iff_definability_memAxiomSetFrameClass (definability : Definability Ax P) : ∀ {W}, [Inhabited W] → ∀ {F}, 𝔽(Ax) W F ↔ P F := by
   apply definability.defines;
 
 
-/-- Every **finite** frame that valid all axioms in `Λ` satisfy **finite** frame property `P` -/
-class FiniteDefinability (Λ : AxiomSet α) (P : FiniteFrameProperty α) where
-  fin_defines : ∀ W, [Inhabited W] → [Finite W] → ∀ F, F ⊧* Λ ↔ @P W _ _ F
+/-- Every **finite** frame that valid all axioms in `Ax` satisfy **finite** frame property `P` -/
+class FiniteDefinability (Ax : AxiomSet α) (P : FiniteFrameProperty α) where
+  fin_defines : ∀ W, [Inhabited W] → [Finite W] → ∀ F, F ⊧* Ax ↔ @P W _ _ F
 
-instance FiniteDefinability.union [definability₁ : FiniteDefinability Λ₁ P₁] [definability₂ : FiniteDefinability Λ₂ P₂] : FiniteDefinability (Λ₁ ∪ Λ₂) (λ F => P₁ F ∧ P₂ F) where
+instance FiniteDefinability.union [definability₁ : FiniteDefinability Ax₁ P₁] [definability₂ : FiniteDefinability Ax₂ P₂] : FiniteDefinability (Ax₁ ∪ Ax₂) (λ F => P₁ F ∧ P₂ F) where
   fin_defines W _ _ F := by
     constructor;
     . intro h;
@@ -232,10 +231,10 @@ instance FiniteDefinability.union [definability₁ : FiniteDefinability Λ₁ P�
       . apply FiniteDefinability.fin_defines W F |>.mpr h.1;
       . apply FiniteDefinability.fin_defines W F |>.mpr h.2;
 
-lemma iff_finiteDefinability_memFiniteFrameClass (definability : FiniteDefinability Λ P) : ∀ {W}, [Inhabited W] → [Finite W] → ∀ {F}, 𝔽ꟳ(Λ) W F ↔ P F := by
+lemma iff_finiteDefinability_memFiniteFrameClass (definability : FiniteDefinability Ax P) : ∀ {W}, [Inhabited W] → [Finite W] → ∀ {F}, 𝔽ꟳ(Ax) W F ↔ P F := by
   apply definability.fin_defines;
 
-instance [definability : Definability Λ P] : FiniteDefinability Λ (λ F => @P _ _ F) where
+instance [definability : Definability Ax P] : FiniteDefinability Ax (λ F => @P _ _ F) where
   fin_defines W _ _ F := by
     constructor;
     . exact iff_definability_memAxiomSetFrameClass definability |>.mp;
@@ -250,36 +249,40 @@ instance {𝔽 : FrameClass α} [ne : FiniteFrameClass.Nonempty (α := α) 𝔽]
     existsi F;
     assumption;
 
+end Kripke
 
-instance AxiomSet.K.definability : Definability (𝐊 : AxiomSet α) (λ _ => True) where
+section K
+
+instance AxiomSet.K.definability : Definability (α := α) 𝗞 (λ _ => True) where
   defines := by
     simp_all;
     intros; subst_vars;
     simp [ValidOnFrame, ValidOnModel, Satisfies];
     intros; simp_all;
 
-instance AxiomSet.K.finiteDefinability : FiniteDefinability (𝐊 : AxiomSet α) (λ _ => True) := inferInstance
+instance AxiomSet.K.finiteDefinability : FiniteDefinability (α := α) 𝗞 (λ _ => True) := inferInstance
 
-instance [definability : Definability Λ P] : Definability (𝐊 ∪ Λ) P := by simpa using Definability.union (definability₁ := AxiomSet.K.definability);
+instance [definability : Definability Ax P] : Definability (𝗞 ∪ Ax) P := by simpa using Definability.union (definability₁ := AxiomSet.K.definability);
 
-instance [definability : FiniteDefinability Λ P] : FiniteDefinability (𝐊 ∪ Λ) P := by simpa using FiniteDefinability.union (definability₁ := AxiomSet.K.finiteDefinability);
+instance [definability : FiniteDefinability Ax P] : FiniteDefinability (𝗞 ∪ Ax) P := by simpa using FiniteDefinability.union (definability₁ := AxiomSet.K.finiteDefinability);
 
-instance : FiniteFrameClass.Nonempty (α := α) 𝔽(𝐊)ꟳ where
+instance : FiniteFrameClass.Nonempty (α := α) 𝔽(𝗞)ꟳ where
   W := PUnit
   existsi := by
     existsi (λ _ _ => True);
     apply iff_finiteDefinability_memFiniteFrameClass AxiomSet.K.finiteDefinability |>.mpr;
     trivial;
 
-instance : FrameClass.Nonempty (α := α) 𝔽(𝐊) := inferInstance
-
+instance : FrameClass.Nonempty (α := α) 𝔽(𝗞) := inferInstance
 
 /- TODO:
-instance [definability : FiniteDefinability Λ P] [nonempty : FiniteFrameClass.Nonempty (α := α) 𝔽(Λ)ꟳ] : FiniteFrameClass.Nonempty 𝔽((𝐊 ∪ Λ))ꟳ where
+instance [definability : FiniteDefinability Ax P] [nonempty : FiniteFrameClass.Nonempty (α := α) 𝔽(Ax)ꟳ] : FiniteFrameClass.Nonempty 𝔽((𝐊 ∪ Ax))ꟳ where
   W := nonempty.W
   W_inhabited := nonempty.W_inhabited
   W_finite := nonempty.W_finite
   existsi := by sorry;
 -/
 
-end LO.Modal.Standard.Kripke
+end K
+
+end LO.Modal.Standard
