Logic/Modal/Standard/Kripke/Soundness.lean
@@ -1,24 +1,24 @@
-import Logic.Modal.Standard.Deduction
 import Logic.Modal.Standard.Kripke.Semantics
+import Logic.Modal.Standard.Deduction
 
 namespace LO.Modal.Standard.Kripke
 
-variable {W α : Type*} {Λ : AxiomSet α}
-variable [Inhabited W] [Inhabited α]
+variable {W α : Type*} [Inhabited W] [Inhabited α]
+variable {L : DeductionParameter α} [L.HasNec]
 
 open Deduction
 open Formula Formula.Kripke
 
-lemma sound_on_frameclass (d : Λ ⊢ p) : 𝔽(Λ) ⊧ p := by
-  induction d with
-  | maxm h => exact validOnAxiomSetFrameClass_axiom h;
-  | mdp _ _ ihpq ihp =>
+lemma sound_on_frameclass (d : L ⊢ p) : 𝔽(Ax(L)) ⊧ p := by
+  induction d using Deduction.inducition_with_nec with
+  | hMaxm h => exact validOnAxiomSetFrameClass_axiom h;
+  | hMdp _ _ ihpq ihp =>
     intro W _ F hF V w;
     exact (Semantics.Tarski.realize_imp.mp $ ihpq W F hF V w) (ihp W F hF V w);
-  | nec _ ih =>
+  | hNec _ ih =>
     intro W _ F hF V w w' _;
     exact ih W F hF V w';
-  | disj₃ =>
+  | hDisj₃ =>
     simp_all [ValidOnFrameClass, ValidOnFrame, ValidOnModel];
     intros; rename_i hpr hqr hpq;
     cases hpq with
@@ -26,11 +26,11 @@ lemma sound_on_frameclass (d : Λ ⊢ p) : 𝔽(Λ) ⊧ p := by
     | inr hq => exact hqr hq;
   | _ => simp_all [ValidOnFrameClass, ValidOnFrame, ValidOnModel];
 
-lemma sound!_on_frameclass : Λ ⊢! p → 𝔽(Λ) ⊧ p := λ ⟨d⟩ => sound_on_frameclass d
+lemma sound!_on_frameclass : L ⊢! p → 𝔽(Ax(L)) ⊧ p := λ ⟨d⟩ => sound_on_frameclass d
 
-instance : Sound Λ (𝔽(Λ)) := ⟨sound!_on_frameclass⟩
+instance : Sound L 𝔽(L.axiomSet) := ⟨sound!_on_frameclass⟩
 
-lemma unprovable_bot [ne : FrameClass.Nonempty 𝔽(Λ)] : Λ ⊬! ⊥ := by
+lemma unprovable_bot [ne : FrameClass.Nonempty 𝔽(Ax(L))] : L ⊬! ⊥ := by
   intro h;
   obtain ⟨F, hF⟩ := ne.existsi;
   have := sound!_on_frameclass h;
@@ -38,11 +38,11 @@ lemma unprovable_bot [ne : FrameClass.Nonempty 𝔽(Λ)] : Λ ⊬! ⊥ := by
   have := @this ne.W ne.W_inhabited F;
   contradiction;
 
-instance [FrameClass.Nonempty 𝔽(Λ)] : System.Consistent Λ := System.Consistent.of_unprovable unprovable_bot
+instance [FrameClass.Nonempty 𝔽(Ax(L))] : System.Consistent L := System.Consistent.of_unprovable unprovable_bot
 
-instance : System.Consistent (𝐊 : AxiomSet α) := inferInstance
+instance : System.Consistent (𝐊 : DeductionParameter α) := inferInstance
 
-lemma unprovable_bot_finite [ne : FiniteFrameClass.Nonempty 𝔽ꟳ(Λ)] : Λ ⊬! ⊥ := by
+lemma unprovable_bot_finite [ne : FiniteFrameClass.Nonempty 𝔽ꟳ(Ax(L))] : L ⊬! ⊥ := by
   intro h;
   obtain ⟨F, hF⟩ := ne.existsi;
   have := sound!_on_frameclass h;
@@ -50,6 +50,6 @@ lemma unprovable_bot_finite [ne : FiniteFrameClass.Nonempty 𝔽ꟳ(Λ)] : Λ �
   have := @this ne.W ne.W_inhabited F;
   contradiction;
 
-instance [FiniteFrameClass.Nonempty 𝔽ꟳ(Λ)] : System.Consistent Λ := System.Consistent.of_unprovable unprovable_bot_finite
+instance [FiniteFrameClass.Nonempty 𝔽ꟳ(Ax(L))] : System.Consistent L := System.Consistent.of_unprovable unprovable_bot_finite
 
 end LO.Modal.Standard.Kripke
